# 第2.2节  微分与切线 - 袁萌专栏 - CSDN博客
2013年07月27日 12:47:45[yuanmeng001](https://me.csdn.net/yuanmeng001)阅读数：1013
2.2 DIFFERENTIALS AND TANGENT LINES
    Suppose we are given a curve* y=f(x)* and at a point (*a, b*) on the curve the slope*f'(a)* is defined.
 Then the tangent line to the curve at the point (*a, b*), illustrated in Figure 2.2.1,is defined to be the straight line which passes through the point (*a,b*) and has the same slope as the curve at*x=a*. Thus the tangent line is given
 by the equation
*l(x) - b = f'(a) (x-a),*
*Or                       l (x)  = f'(a) (x-a)+ b.*
![](http://netdisk0.mail.sina.com.cn/object/f1/2cf1f650e76b2b521dd8a06e78f1278d.files/file0001.png)
![](http://netdisk0.mail.sina.com.cn/object/f1/2cf1f650e76b2b521dd8a06e78f1278d.files/file0002.png)
Figure 2.2.1  Tangent lines
EXAMPLE1 
For the curve*y*=*x*3,find the tangent
 lines at the points (0, 0), (1,1), and (___,____)
(Figure2.2.2). The slope is given by*f*′*(x)* = 3*x²*.At
*x*= 0, *f *′*(*0)=3·0²= 0. The tangent line has the equation
*y*=0(*x*-0)+ 0,  or*y*=0.
![](http://netdisk0.mail.sina.com.cn/object/f1/2cf1f650e76b2b521dd8a06e78f1278d.files/file0003.png)
Figure2.2.2
At *x*= 1,*f*′(1) = 3, whence the tangent line is
*y*=3(*x*-1)+1,   or  *y*=3*x*-2.
At *x*= ____,*f* '(_____)= 3 ·(___)²
 =_____,so the tangent line is
![](http://netdisk0.mail.sina.com.cn/object/f1/2cf1f650e76b2b521dd8a06e78f1278d.files/file0004.png)
Given a curve
*y= f(x)*, suppose that x starts out with the value*a*and then changes by an infinitesimal amountΔ*x*.What happens to*y*? Along the curve,*y*
 will change bythe amount
*f(a+*Δ*x) - f(a) =*Δ*y.*
Butalong the tangent line*y* will change by the amount
*l(a+*Δ*x)- l (a) = [ f*′*(a)(a+*Δ*x-a)+ b] -[ f*′*(a) (a- a) +b]*
*=f *′*(a)*Δ*x.*
When*x* changes from*a* to*a +*Δ*x*,we see that:
change in*y* along curve =*f(a+*Δ*x)- f(a),*
change in*y* along tangent line =*f*′*(a)*Δ*x.*
Inthe last section we introduced the dependent variableΔy,the
 increment of*y*, with the equation
Δ*y*=*f(x +*Δ*x)- f(x).*
Δyis equal to the change in*y*along the curve
 as *x*changes to *x + *Δ*x*.
Thefollowing theorem gives a simple but useful formula for the incrementΔ*y.*
INCREMENT THEOREM
Let *y=f(x)*.Suppose*f*′*(x)*exists at a certain point *x*,and Δ*x*is infinitesimal.
Then Δ*y*is infinitesimal, and
Δ*y*=*f*′*(x)*Δ*x+ ε*Δ*x*
*forsome infinitesimal ε, which depends on x and*Δ*x.*
*PROOF*
Case1  Δ*x*=0.In this case,Δ*y=f*′*(x)*Δ*x*=
 0, and we put*ε*=0.
Case2  Δ*x*≠0 . Then
![](http://netdisk0.mail.sina.com.cn/object/f1/2cf1f650e76b2b521dd8a06e78f1278d.files/file0005.png)
So forsome infinitesimal*ε*,
![](http://netdisk0.mail.sina.com.cn/object/f1/2cf1f650e76b2b521dd8a06e78f1278d.files/file0006.png)
Multiplying both sides by Δ*x*,
Δ*y*=*f*′*(x)*Δ*x + ε* Δ*x.*
EXAMPLE 2  Let*y=x*3, so that*y*′=3*x*2. According tothe Increment Theorem,
Δ*y*=3*x*2 Δ*x* +*ε* Δ*x*
for someinfinitesimal*ε* . Find*ε* in terms of
*x* and Δ*x*when Δ*x*≠ 0. We have
![](http://netdisk0.mail.sina.com.cn/object/f1/2cf1f650e76b2b521dd8a06e78f1278d.files/file0007.png)
We muststill eliminate Δ*y*. From Example 1 in Section 2.1,
![](http://netdisk0.mail.sina.com.cn/object/f1/2cf1f650e76b2b521dd8a06e78f1278d.files/file0008.png)
Substituting,             *ε =*(3*x²+*3*x*Δ*x+*(Δ*x*)²*) -*3*x².*
Since3*x²* cancels,          
*ε=*3*x*Δ*x+*(Δ*x*)²*.*
We shall now introduce a new dependent variable* dy*, called the differential of* y*, with the equation
*dy = f'*′*(x)*Δ*x.*
*dy*is equal to the change in* y* along the tangent line as* x *changes to
*x+ *Δ*x*.In Figure 2.2.3 we see* dy* and
Δ*y* under the microscope.
![](http://netdisk0.mail.sina.com.cn/object/f1/2cf1f650e76b2b521dd8a06e78f1278d.files/file0009.png)
Figure2.2.3
To keep our notation uniform we also introduce the symbol* dx* as another name for
Δ*x*.For an independent variable
*x*,Δ*x*and* dx* are the same, but for a dependent variable* y*. Δ*y *and *dy* are different.
DEFINITION
*Suppose y depends on x, y=f(x).*
*( i) The differential of x is the independent variable dx =*
 Δ*x.*
*(ii) The differential of y is the dependent variable dy given by*
*dy = f'*′*(x)dx.*
When *dx*≠ 0, the equation above may be rewritten as
![](http://netdisk0.mail.sina.com.cn/object/f1/2cf1f650e76b2b521dd8a06e78f1278d.files/file0010.png)
Compare this equation with
![](http://netdisk0.mail.sina.com.cn/object/f1/2cf1f650e76b2b521dd8a06e78f1278d.files/file0011.png)
The quotient* dy/dx* is a very convenient alternative symbol for the derivative
*f‘(x)*. In fact we shall write the derivative in the form*dy/dx*most of the time.
The differential*dy* depends on two independent variables*x* and
*dx*. In functional notation,
*dy = df(x,dx)*
Where*df* is the real function of two variables defined by
*df(x,dx) = f*′*(x)dx.*
When*dx*is substituted for Δ*x* and *dy *for *f*′*(x)dx*, the Increment Theorem takes the short form
Δ*y=dy + ε dx.*
The Increment Theorem can be explained graphically using an infinitesimal microscope. Under an infinitesimal microscope, a line of
 length Δ*x*is magnified to a line of unit length, but a line of length *ε*Δ*x* is only magnified to an infinitesimal length *ε*.Thus the Increment Theorem shows that when*f*′*(x)*exists:
(1) Thedifferential *dy* and the increment Δ*y=dy+ε dx*are so close to each other that they
cannot bedistinguished under an infinitesimal microscope.
(2) the curve *y=f(x)* and the tangent line at (*x,y*) are so closeto each other that they cannot
be distinguished under an infinitesimal microscope; both look like a straight line of
slope *f*′*(x).*
Figure2.2.3 is not really accurate. The curvature had to be exaggerated inorder to distinguish the curve and tangent line under the
 microscope.To give an accurate picture, we need a more complicated figure likeFigure 2.2.4, which has a second infinitesimal microscope trained onthe point (*a+*Δ*x,b+*Δ*y*)in
 the field of view of the original microscope. This secondmicroscope magnifies *ε dx *to a unit length andmagnifies Δ*x*to an infinite length.
![](http://netdisk0.mail.sina.com.cn/object/f1/2cf1f650e76b2b521dd8a06e78f1278d.files/file0012.png)
Figure2.2.4
EXAMPLE3  Whenever a derivative*f*′*(x)*is known, we canfind the differential *dy* at once by simply multiplying thederivative by*dx*, using the formula*dy = f*′*(x)dx*. The examples in the last section give the followingdifferentials.
(a) *y*=*x³*,     *dy* = 3*x²dx.*
(b) *y*=_____,  *dy* =_________ where*x*>0.
(c) *y*=1/*x*,     *dy*=-*dx*/*x*2²     when*x* ≠ 0.
![](http://netdisk0.mail.sina.com.cn/object/f1/2cf1f650e76b2b521dd8a06e78f1278d.files/file0013.png)(d) *y*
 =| *x|*,      *dy*= 
(e)   *y=bt - 16t², dy= (b - 32 t) dt.*
Thedifferential notation may also be used when we are given a system offormulas in which two or more dependent variables depend on
 anindependent variable. For exmple if *y* and *z *arefunctions of *x*,
y*=f(x),   z = g(x),*
ThenΔ*y,*Δ*z, dy , dz* are determined by
Δ*y=f(x+*Δ*x)- f(x),     *Δ*z= g(x+*Δ*x)- g(x),*
*dy =f*′*(x)dx,        dz= g*′*(x) dx.*
*)=*
EXAMPLE 4  Given*y=**___**x,z=x³*, with
*x* as the independent variable , then 
![](http://netdisk0.mail.sina.com.cn/object/f1/2cf1f650e76b2b521dd8a06e78f1278d.files/file0014.png)
Themeaning of the symbols for increment and differential in this examplewill be different if we take*y*as the independent
 variable.Then *x* and *z* are functions of*y*.
*x=2y,    z=8y3.*
NowΔ*y=dy* is just an independent variable, while
![](http://netdisk0.mail.sina.com.cn/object/f1/2cf1f650e76b2b521dd8a06e78f1278d.files/file0015.png)
Moreover,              *dx=2dy, dz=24y² dy.*
Wemay also apply the differential notation to terms. If*l(x)*
 is a term with thevariable x, then *l(x)*determines a function f,
*l(x) =f(x),*
*Andthe differential d( l(x)) has the meaning*
*d(**l(x))= f '(x)dx.*
EXAMPLE5
(a)   *d(x³3) = 3x²**dx.*
![](http://netdisk0.mail.sina.com.cn/object/f1/2cf1f650e76b2b521dd8a06e78f1278d.files/file0016.png)
(b)
![](http://netdisk0.mail.sina.com.cn/object/f1/2cf1f650e76b2b521dd8a06e78f1278d.files/file0017.png)
(c)
![](http://netdisk0.mail.sina.com.cn/object/f1/2cf1f650e76b2b521dd8a06e78f1278d.files/file0018.png)
(d)
(e)   Let *u= bt*and*w=*-16*t²*.Then
*u+w= bt -16t²,  d(u+w) = (b-32t) dt. *
PROBLEMS FOR  SECTION 2.2
InProblems 1-8, express Δ*y*and*dy*asfunctions
 of*x*andΔ*x*,and
 for Δ*x*infinitesimalfind
 an infinitesimal*ε*suchthat
 Δ*y=dy*+*ε*Δ*x.*
1*y=x2                           *2 *y*=-5*x2*
3  ________                4*y=x4 *
5  *y=*1*/x                  *6 *y=x-2*
7  *y=x-*1*/x*8   *y=4x + x3 *
9  If*y*=2*x²*and*z =x³*,find Δ*y,*Δ*z,dy,*and*dz.*
10 If*y*=1/(*x+*1*)*and*z =*1/(*x+2)*,find
 Δ*y, *Δ*z,dy,*and*dz.*
11 Find*d*(2*x*+1)             12 
 Find *d*(*x²**-*3*x)*
13 Find*d*(_______)          14 
 Find *d*(_______)
15 Find*d*(*ax+b*)             16 
 Find *d*(*ax²*)
17 Find*d*(3*+2/x*)             18 
 Find *d*(_______) 
19 Find*d*(_______)           20 
 Find *d*(*x³**- x²*)
21 Let*y*=*_____*,*z=*3*x*.Find*d(y+z)*and*d(y/z).*
22 Let*y*=*x*-1,*z=x³*.Find*d(y+z)*and*d(yz).*
InProblems 23-30 below, find the equation of the line tangent to thegiven curve
 at the given point.
23 *y=x²*;(2,
 4)            24   *y=2x²*;(-1, 2)  
25 *y= -x²*;(0, 0)           26  _____(1,1)
27 *y=*3*x-*4;(1,
 -1)          28 ________(5,2)       
29 *y=x 4*;( -2, 16)          30   *y=x3**-x*;  (
 0, 0)
31 Find the equation of the line tangent
 to the parabola *y= x²*atthe
 point (*x0*,____).
32 Find all points P (*x0*,____)on
 the parabola *y = x²*suchthat the tangent line at*P*passes
through thepoint (0, -4)
□33Prove
 that the line tangent to the parabola *y*=*x²*at*P*(*x*0,____)does
 not meet the 
parabola atany
 point except *P*.
