# 第2.6节  链式规则 - 袁萌专栏 - CSDN博客
2013年07月29日 07:58:28[yuanmeng001](https://me.csdn.net/yuanmeng001)阅读数：1182

2.6 CHAIN RULE
The Chain Rule is more general than the Inverse Function Rule and deals with the case where*x* and
*y* are both functions of a third variable *t.*
Suppose            *x= f(t),   y=G(x).*
Thus* x* depends on*t*, and
*y* depends on *x*. But *y* is also a function of*t*.
*y=g(t),*
Where*g*is defined by the rule            *g(t)=G(f(t)).*
Thefunction*g* is sometimes called the composition of
*G* and*f *(sometimes written*g = G ° f ).*
Thecomposition of*G*and*f*maybe
 described in terms of black boxes. The function*g=G° f  *isa large black box operating on the input*t*toproduce*g(t)=G(f(t)).*Ifwe
 look inside this black box (pictured in Figure 2.6.1), we see twosmaller black boxes,*f*and*G*.First*f*operateson
 the input*t*toproduce*f(t)*,and then*G*operateson*f(t)*toproduce the final output*g(t)= G(f(t)).*
TheChain Rule expresses the derivative of*g*interms
 of the derivatives of*f*and*G.*Itleads
 to the powerful method of“changeof variables”incomputing
 derivatives and ,later on, integrals.
![](https://img-blog.csdn.net/20130731143529203?watermark/2/text/aHR0cDovL2Jsb2cuY3Nkbi5uZXQveXVhbm1lbmcwMDE=/font/5a6L5L2T/fontsize/400/fill/I0JBQkFCMA==/dissolve/70/gravity/SouthEast)
Figure2.6.1
CHAIN RULE
*Let f,G be two real functions and define the new function g by the rule*
*g(t)= G(f(t)).*
*At anyvalue of t where the derivatives f '(t) and G'(f(t)) exist, g'(t) also exists and has the value*
*g'(t) = G'(f(t)) f '(t).*
*PROOF Let                     x=f(t),   y=g(t),   y=G(x).*
*Take tas the independent variable, and let*Δ*t*≠*0 be infinitesimal. Form the corresponding increments *Δ*xand*Δ*y.By the Increment Theorem for x=f(t),*Δ*xis infinitesimal. Using the Increment Theorem again but this time fory=G(x), we have*
Δy*=G*′*(x)*Δ*x+ε*Δ*x*
*For someinfinitesimal ε. Dividing by*Δ*t,*
![](http://netdisk0.mail.sina.com.cn/object/10/30100e357113d6f1d0ba9a6ab5749934.files/file0014.png)
*Then takingstandard parts,*
![](http://netdisk0.mail.sina.com.cn/object/10/30100e357113d6f1d0ba9a6ab5749934.files/file0015.png)
*or                 g*′*(t) = G*′*(x) f*′*(t) = G*′*(f(t))f *′*(t).*
![](https://img-blog.csdn.net/20130731143621984?watermark/2/text/aHR0cDovL2Jsb2cuY3Nkbi5uZXQveXVhbm1lbmcwMDE=/font/5a6L5L2T/fontsize/400/fill/I0JBQkFCMA==/dissolve/70/gravity/SouthEast)
EXAMPLE 1 Find the derivative of*g(t) =*1n*(sin t). G(t)*isthe natural logarithm of the sine of*t.*
Itcan be written in the form.
*g(t) =G(f(t))*
Where*f(t) =*sin*t,         G(x) =*1n*x.*
We have *f '(t) = cos t,       *
*Bythe Chain Rule,*
![](https://img-blog.csdn.net/20130731143745781?watermark/2/text/aHR0cDovL2Jsb2cuY3Nkbi5uZXQveXVhbm1lbmcwMDE=/font/5a6L5L2T/fontsize/400/fill/I0JBQkFCMA==/dissolve/70/gravity/SouthEast)
EXAMPLE 2   Find the derivative of*g(t)*=_________________.*g(t)*hasthe
 form
*g(t)= G(f(t)),*
Where    *f(t) = 3t + 1,*G(x)=__________.
We have   *f*′*(t)*=3,     ________________.
![](https://img-blog.csdn.net/20130731143826406?watermark/2/text/aHR0cDovL2Jsb2cuY3Nkbi5uZXQveXVhbm1lbmcwMDE=/font/5a6L5L2T/fontsize/400/fill/I0JBQkFCMA==/dissolve/70/gravity/SouthEast)
Then      
*Inpractice it is more convenient to use the Chain Rule with dependentvariables x and y instead of functions f and g.*
CHAIN RULE  WITH  DEPENDENT  VARIABLES
*Let               x= f(t),    y=g(t) = G(x).*
*Assumeg'(t) and G'(x) exist. Then*
![](https://img-blog.csdn.net/20130731143902218?watermark/2/text/aHR0cDovL2Jsb2cuY3Nkbi5uZXQveXVhbm1lbmcwMDE=/font/5a6L5L2T/fontsize/400/fill/I0JBQkFCMA==/dissolve/70/gravity/SouthEast)
*Wheredx/dt, dy/dt are computed with t as the independent variable, anddy/dx is computed with x as the independent variable.*
Letus work Examples 1 and 2 again with dependent variables.
EXAMPLE 1  (Continued)*Let x=sin t,   y=1nx.*
Find *dy/dt*usingChain
 Rule (i) and *dy *byusing Chain Rule (ii).
(i)               ![](https://img-blog.csdn.net/20130731143934843?watermark/2/text/aHR0cDovL2Jsb2cuY3Nkbi5uZXQveXVhbm1lbmcwMDE=/font/5a6L5L2T/fontsize/400/fill/I0JBQkFCMA==/dissolve/70/gravity/SouthEast)
(ii)![](https://img-blog.csdn.net/20130731144005406?watermark/2/text/aHR0cDovL2Jsb2cuY3Nkbi5uZXQveXVhbm1lbmcwMDE=/font/5a6L5L2T/fontsize/400/fill/I0JBQkFCMA==/dissolve/70/gravity/SouthEast)
EXAMPLE 2  (Continued)  Let*x*=3*t*+1,   
 y=______
![](https://img-blog.csdn.net/20130731145436406?watermark/2/text/aHR0cDovL2Jsb2cuY3Nkbi5uZXQveXVhbm1lbmcwMDE=/font/5a6L5L2T/fontsize/400/fill/I0JBQkFCMA==/dissolve/70/gravity/SouthEast)
(i)
![](http://netdisk0.mail.sina.com.cn/object/10/30100e357113d6f1d0ba9a6ab5749934.files/file0023.png)(ii)
![](http://netdisk0.mail.sina.com.cn/object/10/30100e357113d6f1d0ba9a6ab5749934.files/file0024.png)The equation
![](https://img-blog.csdn.net/20130731145533765?watermark/2/text/aHR0cDovL2Jsb2cuY3Nkbi5uZXQveXVhbm1lbmcwMDE=/font/5a6L5L2T/fontsize/400/fill/I0JBQkFCMA==/dissolve/70/gravity/SouthEast)
With*t*asthe
 independent variable is trivial. We simply cancel the*dx*’s.But when*dy/dx*iscomputed with*x*asthe independent variable while*dx/dt*iscomputed with*t*asthe
 independent variable, the two*dx*’shave different meanings, and the equation is not trivial.
Similarly, the equation
![](https://img-blog.csdn.net/20130731150948046?watermark/2/text/aHR0cDovL2Jsb2cuY3Nkbi5uZXQveXVhbm1lbmcwMDE=/font/5a6L5L2T/fontsize/400/fill/I0JBQkFCMA==/dissolve/70/gravity/SouthEast)
istrivial with*x*asthe
 independent variable but not when*t *isthe independent variable in*dy*and*dx,*while*x*isindependent
 in*dy/dx.*
TheChain Rule shows that when we change independent variables the equations
![](https://img-blog.csdn.net/20130731151018046?watermark/2/text/aHR0cDovL2Jsb2cuY3Nkbi5uZXQveXVhbm1lbmcwMDE=/font/5a6L5L2T/fontsize/400/fill/I0JBQkFCMA==/dissolve/70/gravity/SouthEast)
remaintrue.
TheInverse Function Rule can be proved from the Chain Rule as follows 
Let
*y=f(x),   x=g(y)*
beinverse functions whose derivatives exist. Then
![](https://img-blog.csdn.net/20130731151101421?watermark/2/text/aHR0cDovL2Jsb2cuY3Nkbi5uZXQveXVhbm1lbmcwMDE=/font/5a6L5L2T/fontsize/400/fill/I0JBQkFCMA==/dissolve/70/gravity/SouthEast)
Whence                       
Usingthe Chain Rule we may write the Power Rule in a general form.
POWER RULE
Let*r*bea
 rational number, and let *u*dependon*x*.If*u*>0 and*du/dx*exists,then
![](https://img-blog.csdn.net/20130731151141750?watermark/2/text/aHR0cDovL2Jsb2cuY3Nkbi5uZXQveXVhbm1lbmcwMDE=/font/5a6L5L2T/fontsize/400/fill/I0JBQkFCMA==/dissolve/70/gravity/SouthEast)
Thisis proved by letting*y=u r*andcomputing*dy/ dx*bythe Chain Rule,
![](https://img-blog.csdn.net/20130731151233796?watermark/2/text/aHR0cDovL2Jsb2cuY3Nkbi5uZXQveXVhbm1lbmcwMDE=/font/5a6L5L2T/fontsize/400/fill/I0JBQkFCMA==/dissolve/70/gravity/SouthEast)
TheChain Rule has two types of applications.
(1)Given*x=f(t)*and*y=G(x)*,find___.Use________.
(2)Given*x=f(t)*and*y=g(t)*,find___.Use________.
![](https://img-blog.csdn.net/20130731151304765?watermark/2/text/aHR0cDovL2Jsb2cuY3Nkbi5uZXQveXVhbm1lbmcwMDE=/font/5a6L5L2T/fontsize/400/fill/I0JBQkFCMA==/dissolve/70/gravity/SouthEast)
Applicationsof type (1) often arise when a new dependent variable*x*isintroduced
 to help compute___.Applicationsof
 type (2) arise when two variables *x*and*y*bothdepend
 on a third variable*t*,for example, when*x*and*y*arethe
 coordinates of a moving particle and*t *istime.
Wegive three examples of type (1) and then two of type (2).
EXAMPLE 3  Suppose that by investing*t*dollarsa company can produce
![](https://img-blog.csdn.net/20130731151344046?watermark/2/text/aHR0cDovL2Jsb2cuY3Nkbi5uZXQveXVhbm1lbmcwMDE=/font/5a6L5L2T/fontsize/400/fill/I0JBQkFCMA==/dissolve/70/gravity/SouthEast)
Items,and that it can sell*x*itemsfor
 a total profit of
![](https://img-blog.csdn.net/20130731151508437?watermark/2/text/aHR0cDovL2Jsb2cuY3Nkbi5uZXQveXVhbm1lbmcwMDE=/font/5a6L5L2T/fontsize/400/fill/I0JBQkFCMA==/dissolve/70/gravity/SouthEast)
Find___,which
 is the marginal profit with respect to the amount invested.
![](https://img-blog.csdn.net/20130731151554203?watermark/2/text/aHR0cDovL2Jsb2cuY3Nkbi5uZXQveXVhbm1lbmcwMDE=/font/5a6L5L2T/fontsize/400/fill/I0JBQkFCMA==/dissolve/70/gravity/SouthEast)
Wehave         
![](http://netdisk0.mail.sina.com.cn/object/10/30100e357113d6f1d0ba9a6ab5749934.files/file0034.png)Bythe
 Chain Rule,
Thusafter*t*dollarshave been invested, an additional dollar invested will bring 0.7 -*t/*5000dollars of additional
 profit.
EXAMPLE4  Find*dy/dt*where*y*=(5t²-2) 1/4 .
Let                *x*=5*t*²-2 *y*=*x*1/4.
![](https://img-blog.csdn.net/20130731151657968?watermark/2/text/aHR0cDovL2Jsb2cuY3Nkbi5uZXQveXVhbm1lbmcwMDE=/font/5a6L5L2T/fontsize/400/fill/I0JBQkFCMA==/dissolve/70/gravity/SouthEast)
Then 
EXAMPLE 5 
Find*dy/dx*where ![](http://netdisk0.mail.sina.com.cn/object/10/30100e357113d6f1d0ba9a6ab5749934.files/file0036.png)
Thisproblem requires three uses of the Chain Rule.
![](http://netdisk0.mail.sina.com.cn/object/10/30100e357113d6f1d0ba9a6ab5749934.files/file0037.png)Let         
Thenby the Chain Rule,
![](http://netdisk0.mail.sina.com.cn/object/10/30100e357113d6f1d0ba9a6ab5749934.files/file0038.png)
Nowlet*v*=sin(4*x*+1),*w*=cos(4*x*-1),*u=v + w.*
![](http://netdisk0.mail.sina.com.cn/object/10/30100e357113d6f1d0ba9a6ab5749934.files/file0039.png)
Then           
![](https://img-blog.csdn.net/20130731151755437?watermark/2/text/aHR0cDovL2Jsb2cuY3Nkbi5uZXQveXVhbm1lbmcwMDE=/font/5a6L5L2T/fontsize/400/fill/I0JBQkFCMA==/dissolve/70/gravity/SouthEast)
Weuse the Chain Rule twice more to find*dv/dx*and*dw/dx.*
![](https://img-blog.csdn.net/20130731151853265?watermark/2/text/aHR0cDovL2Jsb2cuY3Nkbi5uZXQveXVhbm1lbmcwMDE=/font/5a6L5L2T/fontsize/400/fill/I0JBQkFCMA==/dissolve/70/gravity/SouthEast)
Finally,we combine everything to get
![](https://img-blog.csdn.net/20130731151940109?watermark/2/text/aHR0cDovL2Jsb2cuY3Nkbi5uZXQveXVhbm1lbmcwMDE=/font/5a6L5L2T/fontsize/400/fill/I0JBQkFCMA==/dissolve/70/gravity/SouthEast)
Ifa particle is moving in the plane, its position
 (*x,y*)at time t will be given by a pair of equations
*x=f(t), y=g(t).*
Theseare called*parametric equations. *Theslope of the curve traced out by this particle can be found by theChain Rule,
![](https://img-blog.csdn.net/20130731152010203?watermark/2/text/aHR0cDovL2Jsb2cuY3Nkbi5uZXQveXVhbm1lbmcwMDE=/font/5a6L5L2T/fontsize/400/fill/I0JBQkFCMA==/dissolve/70/gravity/SouthEast)
Wheneverthe derivatives exist and*f '(t) *≠ *0. Thisis a Chain Rule application of type (2).*
EXAMPLE 6 
Aball thrown horizontally from a 100 ft cliff at a velocity of 50ft/sec will follow the parametric equations
x=50*t*,*y*=100-16*t*², in
 feet.
Findthe slope of its path at time*t*(Figure
 2.6.2).
So             
![](https://img-blog.csdn.net/20130731152059687?watermark/2/text/aHR0cDovL2Jsb2cuY3Nkbi5uZXQveXVhbm1lbmcwMDE=/font/5a6L5L2T/fontsize/400/fill/I0JBQkFCMA==/dissolve/70/gravity/SouthEast)
![](https://img-blog.csdn.net/20130731152135562?watermark/2/text/aHR0cDovL2Jsb2cuY3Nkbi5uZXQveXVhbm1lbmcwMDE=/font/5a6L5L2T/fontsize/400/fill/I0JBQkFCMA==/dissolve/70/gravity/SouthEast)
Figure2.6.2
EXAMPLE7  A particle moves according to the
 parametric equations
*x*=*t³*-*t*, *y=t²*.
Find the slope of its path.
![](https://img-blog.csdn.net/20130731152249484?watermark/2/text/aHR0cDovL2Jsb2cuY3Nkbi5uZXQveXVhbm1lbmcwMDE=/font/5a6L5L2T/fontsize/400/fill/I0JBQkFCMA==/dissolve/70/gravity/SouthEast)
So         
Wesee from Figure 2.6.3 that the path of this
 particle is not the graphof a function, and in fact contains a loop and crosses the point(0,1) twice, at*t*=-1 and*t*=1. The path is vertical at the points t=______,where
 there is no slope. At the point (0,1), the two slopes of thepath are *dy/dx*=-1 when*t*=-1,
 and*dy/dx*=1 when*t*=1.
EXAMPLE8 A particle moving according to the
 parametric equations
*x*=cos*t*, *y*=sin*t*
Will movecounterclockwise around the unit circle at one radian per second
![](https://img-blog.csdn.net/20130731152357046?watermark/2/text/aHR0cDovL2Jsb2cuY3Nkbi5uZXQveXVhbm1lbmcwMDE=/font/5a6L5L2T/fontsize/400/fill/I0JBQkFCMA==/dissolve/70/gravity/SouthEast)
Figure2.6.3
beginning atthe
 point (1,0), as shown in Figure 2.6.4. Find the slope of its pathat time *t*.
![](https://img-blog.csdn.net/20130731152457796?watermark/2/text/aHR0cDovL2Jsb2cuY3Nkbi5uZXQveXVhbm1lbmcwMDE=/font/5a6L5L2T/fontsize/400/fill/I0JBQkFCMA==/dissolve/70/gravity/SouthEast)
Theslope is
![](https://img-blog.csdn.net/20130731152506062?watermark/2/text/aHR0cDovL2Jsb2cuY3Nkbi5uZXQveXVhbm1lbmcwMDE=/font/5a6L5L2T/fontsize/400/fill/I0JBQkFCMA==/dissolve/70/gravity/SouthEast)
Interms of x and y the slope is
![](https://img-blog.csdn.net/20130731152552843?watermark/2/text/aHR0cDovL2Jsb2cuY3Nkbi5uZXQveXVhbm1lbmcwMDE=/font/5a6L5L2T/fontsize/400/fill/I0JBQkFCMA==/dissolve/70/gravity/SouthEast)
![](https://img-blog.csdn.net/20130731152629890?watermark/2/text/aHR0cDovL2Jsb2cuY3Nkbi5uZXQveXVhbm1lbmcwMDE=/font/5a6L5L2T/fontsize/400/fill/I0JBQkFCMA==/dissolve/70/gravity/SouthEast)
Figure 2.6.4
