# 第2.4节  反函数 - 袁萌专栏 - CSDN博客
2013年07月27日 15:29:41[yuanmeng001](https://me.csdn.net/yuanmeng001)阅读数：1050
2.4 INVERSE FUNCTIONS
Two real functions
*f *and *g* are called *inverse functions *if the two equations
*y=f(x),  x=g(y)*
Have the same graphs in the (*x, y*) plane. That is, a point (*x,y*) is on the curve
*y=f(x)* if, and only if, it is on the curve *x=g(y).* (in general, the graph of the equation
*x=g(y)*is different from the graph of *y=g(x)*, but is the same asthe graph of
*y=f(x)*; see Figure 2.4.1.)
![](http://netdisk0.mail.sina.com.cn/object/92/db926dafde7f1d190f839e07d19a9567.files/file0040.png)
![](http://netdisk0.mail.sina.com.cn/object/92/db926dafde7f1d190f839e07d19a9567.files/file0041.png)

Figure2.4.1 inverse functions
Forexample, the function
*y=x², x *≥ 0, has the inverse function*x*=_______; the function
*y=x *³has the inverse function
*x*=______.
Ifwe think of f as a black box operating on an input
*x *toproduce an output *f(x)*, the inverse function *g* is ablack box operating on the output
*f(x)* to undo the work of *f*and produce the original input *x *(see Figure 2.4.2).
![](http://netdisk0.mail.sina.com.cn/object/92/db926dafde7f1d190f839e07d19a9567.files/file0042.png)
Figure2.4.2
Manyfunctions, such as
*y=x*2, do not have inverse functions. InFigure 2.4.3, we see that *x *
is not a function of *y*because at *y*=1, *x* has the two values
*x*=1 and *x*=-1.
Oftenone can tell whether a function
*f* has an inverse by looking atits graph. If there is a horizontal line *y=c *which cuts thegraph at more than one point, the function *f *has no inverse.(see figure 2.4.3.) if no horizontal line cuts the graph at more thanone point, then
*f* has an inverse function g. Using this rule,we can see in figure 2.4.4 that the functions
*y=| x |*and *y* = _______________ 
do nothave inverses.
![](http://netdisk0.mail.sina.com.cn/object/92/db926dafde7f1d190f839e07d19a9567.files/file0043.png)

Figure2.4.3
![](http://netdisk0.mail.sina.com.cn/object/92/db926dafde7f1d190f839e07d19a9567.files/file0044.png)
![](http://netdisk0.mail.sina.com.cn/object/92/db926dafde7f1d190f839e07d19a9567.files/file0045.png)Figure 2.4.4                  No
 inverse functions
Table2.4.1 shows some familiar functions which do have inverses.
![](http://netdisk0.mail.sina.com.cn/object/92/db926dafde7f1d190f839e07d19a9567.files/file0046.png)Notethat
 in each case, 
![](http://netdisk0.mail.sina.com.cn/object/92/db926dafde7f1d190f839e07d19a9567.files/file0047.png)

Supposethe (*x, y*) plane is flipped over about the diagonal line
*y=x*.This will make the *x*-and *y*-axes change places, formingthe (*y,x*) plane. If f has an inverse function
*g*, thegraph of the function *y=f(x)* will become the graph of theinverse function
*x=g(y)* in the (*y, x*) plane, as shownin Figure 2.4.5.
Thefollowing rule shows that the derivatives of inverse functions arealways reciprocals of each other.
INVERSE FUNCTION  RULE
*Suppose fand g are inverse functions, so that the two equations*
*y=f(x)    and    x=g(y)*
*have thesame graphs. If both derivatives f '(x) and g '(y) exist and arenonzero,*
![](http://netdisk0.mail.sina.com.cn/object/92/db926dafde7f1d190f839e07d19a9567.files/file0048.png)
then                     
![](http://netdisk0.mail.sina.com.cn/object/92/db926dafde7f1d190f839e07d19a9567.files/file0049.png)
thatis,    
PROOF Let Δ*x* be a nonzero infinitesimal and let Δy be thecorresponding change in
*y*. Then Δy is also infinitesimalbecause *f '(x) *exists and is nonzero because
*f(x)* hasan inverse function. By the rules for standard parts,
![](http://netdisk0.mail.sina.com.cn/object/92/db926dafde7f1d190f839e07d19a9567.files/file0050.png)
![](http://netdisk0.mail.sina.com.cn/object/92/db926dafde7f1d190f839e07d19a9567.files/file0051.png)Therefore  
![](http://netdisk0.mail.sina.com.cn/object/92/db926dafde7f1d190f839e07d19a9567.files/file0052.png)
![](http://netdisk0.mail.sina.com.cn/object/92/db926dafde7f1d190f839e07d19a9567.files/file0053.png)
(a)
![](http://netdisk0.mail.sina.com.cn/object/92/db926dafde7f1d190f839e07d19a9567.files/file0054.png)![](http://netdisk0.mail.sina.com.cn/object/92/db926dafde7f1d190f839e07d19a9567.files/file0055.png)
(b)
![](http://netdisk0.mail.sina.com.cn/object/92/db926dafde7f1d190f839e07d19a9567.files/file0056.png)![](http://netdisk0.mail.sina.com.cn/object/92/db926dafde7f1d190f839e07d19a9567.files/file0057.png)
(c)
![](http://netdisk0.mail.sina.com.cn/object/92/db926dafde7f1d190f839e07d19a9567.files/file0058.png)![](http://netdisk0.mail.sina.com.cn/object/92/db926dafde7f1d190f839e07d19a9567.files/file0059.png)
(d)
Figure2.4.5
![](http://netdisk0.mail.sina.com.cn/object/92/db926dafde7f1d190f839e07d19a9567.files/file0060.png)Theformula
inthe Inverse Function Rule is not as trivial as it looks. A morecomplete statement is
____ computed with
*x* the independent variable
=________ computed with y the independentvariabe.
Sometimesit is easier to compute
*dx/dy* than *dy/dx*, and in suchcases the Inverse Function Rule is a useful method.
EXAMPLE1  Find
*dy/dx *where *x*=1+*y* -3.
Before solvingthe problem we note that
![](http://netdisk0.mail.sina.com.cn/object/92/db926dafde7f1d190f839e07d19a9567.files/file0061.png)
So *x*and
*y* are inverse functions of each other. We want to find
![](http://netdisk0.mail.sina.com.cn/object/92/db926dafde7f1d190f839e07d19a9567.files/file0062.png)
With*x* the independent variable. This looks hard, but it is easy tocompute
![](http://netdisk0.mail.sina.com.cn/object/92/db926dafde7f1d190f839e07d19a9567.files/file0063.png)
With*y*theindependent variable.
SOLUTION  ____ = -3*y*-4,
![](http://netdisk0.mail.sina.com.cn/object/92/db926dafde7f1d190f839e07d19a9567.files/file0064.png)
Wecan write
*dy/dx* in terms of *x *by substituting,
![](http://netdisk0.mail.sina.com.cn/object/92/db926dafde7f1d190f839e07d19a9567.files/file0065.png)
EXAMPLE 2  Find
*dy/dx *where *x*= *y*5 + *y*3 + y.Compute *dy/dx *
at the point(3,1).
Although wecannot solve the equation explicitly for
*y* as a function of *x*,we can see from the graph in Figure 2.4.6 that there is an inversefunction
*y=f(x).*
![](http://netdisk0.mail.sina.com.cn/object/92/db926dafde7f1d190f839e07d19a9567.files/file0066.png)![](http://netdisk0.mail.sina.com.cn/object/92/db926dafde7f1d190f839e07d19a9567.files/file0067.png)

Figure2.4.6
Bythe Inverse Function Rule,
![](http://netdisk0.mail.sina.com.cn/object/92/db926dafde7f1d190f839e07d19a9567.files/file0068.png)
Thistime we must leave the answer in term of
*y*. At the point(3,1), we substitute 1 for *y* and get *dy/dx* = 1/9.
Fory≥ 0, the function
*x= y n* has the inverse function *y=x1/n*. In the next theorem, we use the Inverse Function Rule tofind a new derivative, that of
*y= x1/n*. 
THEOREM 1
*If nis a positive integer and*
*y=x1/n*.
![](http://netdisk0.mail.sina.com.cn/object/92/db926dafde7f1d190f839e07d19a9567.files/file0069.png)then                   
Rememberthat
*y= x1/n*. is defined for all *x* if n is odd and for *x* > 0 if
*n* is even. 
Thederivative______ is defined for
*x*≠0 if *n *is odd and for *x *> 0 if *n* is even.
Ifwe are willing to assume that
*dy/ dx* exists, then we canquickly find *dy/dx *by the Inverse Function Rule.
![](http://netdisk0.mail.sina.com.cn/object/92/db926dafde7f1d190f839e07d19a9567.files/file0070.png)
Hereis a longer but complete proof which shows that
*dy/dx* existsand computes its value.
PROOF OF  THEOREM 1
Let *x*≠0 and let Δ*x*be nonzero infinitesimal. We first show that
Δ*y*=(*x +*Δ*x*)1/n -
*x*1/n
is anonzero infinitesimal. Δ*y* ≠ 0 because
*x+*Δ*x*≠ *x*. The standard part of 
Δ*y*is
*st(*Δ*y) = st(( x+* Δ
*x)*1/n*) - st(x*1/n *)*
*=x*1/n*- x*1/n
*= *0*.*
Therefore*y* is nonzero infinitesimal.
![](http://netdisk0.mail.sina.com.cn/object/92/db926dafde7f1d190f839e07d19a9567.files/file0071.png)Now                  
![](http://netdisk0.mail.sina.com.cn/object/92/db926dafde7f1d190f839e07d19a9567.files/file0072.png)
Therefore
![](http://netdisk0.mail.sina.com.cn/object/92/db926dafde7f1d190f839e07d19a9567.files/file0073.png)
![](http://netdisk0.mail.sina.com.cn/object/92/db926dafde7f1d190f839e07d19a9567.files/file0074.png)
Figure2.4.7
Figure2.4.7 shows the graphs of
*y*=*x*1/3 and *y*=*x*1/4.At *x* =0, the curves are vertical and have no slope.
EXAMPLE 3  Find the derivatives of
*y*=*x*1/n for *n*=2,3,4.
![](http://netdisk0.mail.sina.com.cn/object/92/db926dafde7f1d190f839e07d19a9567.files/file0075.png)
UsingTheorem 1 we can show that the Power Rule holds when the exponent isany rational number.
POWER RULE  FOR  RATIONAL  EXPONENTS
*Lety=xr where r is a rational number. Then whenever x>0,*
![](http://netdisk0.mail.sina.com.cn/object/92/db926dafde7f1d190f839e07d19a9567.files/file0076.png)
PROOF Let
*r=m/n* where *m* and *n* are integers, *n*>0.Let
*u=x1/n,  y=um.*
Then               __________________
![](http://netdisk0.mail.sina.com.cn/object/92/db926dafde7f1d190f839e07d19a9567.files/file0077.png)and
EXAMPLE 4  Find
*dy/dx* where
![](http://netdisk0.mail.sina.com.cn/object/92/db926dafde7f1d190f839e07d19a9567.files/file0078.png)
EXAMPLE 5  Find
*dy/dx *where
______________________.
Let               *u=2+x*3/2*,  y= u*-1.
![](http://netdisk0.mail.sina.com.cn/object/92/db926dafde7f1d190f839e07d19a9567.files/file0079.png)Then          
PROBLEMS FOR  SECTION 2.4
InProblems 1-16, find dy/dx.
1     *x=3y3 + 2y                    *2*x = y2 +*1*,   y>0*
3      *x=*1-*2y2 , y>0                 *4  *x*=2*y5*+*y3*+4
5      *x= (y2 +2)-1 , y>0                6  **_______*
7      *y=x*4/3                                8  _______
9     ____________  10 *y= (2x *1/3+1)3 
11     *y=*1*+2x*1/3+ 4*x*2/3+6*x*12 *y=x*-1/4*+*3*x *-3/4
13     *y=*(*x*5/3-
*x) *-2                          14  
*x=**y*+_____
15    *x=*3*x*1/3+*2y,  y*>0              16     
*x=*1/(1+
____*)*
InProblems 17-25, find the inverse function
*y* and its derivative*dy/dx* as functions of *x*.
17  *x=ky+c,  k*≠ 0                    18   
*x*= *y*3 + 1
19   *x*=2*y*2+1, y≥ 0                     20   
*x*=2*y*2+1, y≤0    
21   *x*=*y*4 - 3, y≥ 0                      22   
*x*=*y*2+3*y*-1,  y ≥ ____
23   *x*=*y*4+*y*2
*+*1, y≥ 0                   24   x = 1/*y*2 +1/*y -*1,  y > 0  
25  _______________
□26 show that no second degree polynomial
*x= ay2 + by +c*has an inverse function.
□27 show that
*x=ay2 + by + c, y *≥ *-b/2a*, has aninverse function. What does its graph look
like?
□28 Prove that a function
*y=f(x) *has an inverse function if andonly if whenever *x1*≠ *x2,*
*f(x1)__f(x2)  *
